theories/filter.v
@@ -15,6 +15,10 @@ Inductive filter_step {EV1 EV2} (m : module EV1) (R : EV1 → option EV2 → Pro
 Definition mod_filter {EV1 EV2} (m : module EV1) (R : EV1 → option EV2 → Prop) : module EV2 :=
   Mod (filter_step m R).
 
+Global Instance filter_vis_no_all {EV1 EV2} (m : module EV1) (R : EV1 → option EV2 → Prop) `{!VisNoAll m}:
+  VisNoAll (mod_filter m R).
+Proof. move => *. invert_all @m_step; case_match; simplify_eq. by apply: vis_no_all. Qed.
+
 Module filter_example.
   (* This example shows that filter does not preserve refinement if
   the filter function is not functional, i.e. if it can introduce
